theories/examples/awkward_example_extra.v
@@ -1,4 +1,4 @@
-From iris.proofmode Require Import tactics.
+From iris.proofmode Require Import proofmode.
 From iris.base_logic Require Import invariants.
 Require Import Eqdep_dec.
 From cap_machine Require Import
@@ -8,7 +8,7 @@ From cap_machine Require Export stdpp_extra iris_extra.
 
 Section awkward_helpers.
   Context {Σ:gFunctors} {memg:memG Σ} {regg:regG Σ}
-          {stsg : STSG Addr region_type Σ} {heapg : heapG Σ}
+          {stsg : STSG Addr region_type Σ} {heapg : heapGS Σ}
           {nainv: logrel_na_invs Σ}
           `{MP: MachineParameters}.
 
